MasterThesis/SCORE/Test/Compiler.lean
@@ -5,7 +5,7 @@ open SCORE
 
 def store0 : Store := ["x" ↦ [0]] ["y" ↦ [3]] ["z" ↦ [0]]
 
-def storePred : Store := (eval (L2S LOOP.func.pred) store0)
+def storePred : Store := (eval (l2s LOOP.func.pred) store0)
 #eval  storePred "x"
-def storePredᵢ : Store := (evalI (L2S LOOP.func.pred) storePred)
+def storePredᵢ : Store := (evalI (l2s LOOP.func.pred) storePred)
 #eval storePredᵢ "y"
